% Generated on 2023-07-17 16:54:29 by gEcon ver. 1.2.1 (2023-01-18)
% http://gecon.r-forge.r-project.org/

% Model name: RSW

\section{HIGHREGIME}

\subsection{Optimisation problem}

\begin{align}
&\max_{{p\!i\!H}_{t}, {y\!H}_{t}, {i\!H}_{t}
} {U\!H}_{t} = -0.5{{p\!i\!H}_{t}}^{2} + {\beta} \left({{p\!H}} {\mathrm{E}_{t}\left[{U\!H}_{t+1}\right]} + \left(1 - {p\!H}\right) {\mathrm{E}_{t}\left[{U\!L}_{t+1}\right]}\right) - 0.5{\kappa} {\theta}^{-1} {{y\!H}_{t}}^{2}\\
&\mathrm{s.t.:}\nonumber\\
& {p\!i\!H}_{t-1} = {\beta} \left({{p\!H}} {{p\!i\!H}_{t}} + {{p\!i\!L}_{t}} \left(1 - {p\!H}\right)\right) + {\kappa} {{y\!H}_{t-1}} \quad \left(\lambda^{\mathrm{HIGHREGIME}^{\mathrm{1}}}_{t}\right)\\
& {y\!H}_{t-1} = {{p\!H}} {{y\!H}_{t}} + {{y\!L}_{t}} \left(1 - {p\!H}\right) - {\sigma} \left({i\!H}_{t-1} - {r\!n}_{t-1} - {{p\!H}} {{p\!i\!H}_{t}} - {{p\!i\!L}_{t}} \left(1 - {p\!H}\right)\right) \quad \left(\lambda^{\mathrm{HIGHREGIME}^{\mathrm{2}}}_{t}\right)
\end{align}


\subsection{First order conditions}

\begin{equation}
-{p\!i\!H}_{t} + {\beta} {{p\!H}} {\lambda^{\mathrm{HIGHREGIME}^{\mathrm{1}}}_{t}} - {\beta} {{p\!H}} {\mathrm{E}_{t}\left[\lambda^{\mathrm{HIGHREGIME}^{\mathrm{1}}}_{t+1}\right]} + {{p\!H}} {\sigma} {\lambda^{\mathrm{HIGHREGIME}^{\mathrm{2}}}_{t}} = 0
 \quad \left({p\!i\!H}_{t}\right)
\end{equation}
\begin{equation}
{{p\!H}} {\lambda^{\mathrm{HIGHREGIME}^{\mathrm{2}}}_{t}} + {\beta} {{p\!H}} \left({\kappa} {\mathrm{E}_{t}\left[\lambda^{\mathrm{HIGHREGIME}^{\mathrm{1}}}_{t+1}\right]} - \mathrm{E}_{t}\left[\lambda^{\mathrm{HIGHREGIME}^{\mathrm{2}}}_{t+1}\right]\right) - {\kappa} {\theta}^{-1} {{y\!H}_{t}} = 0
 \quad \left({y\!H}_{t}\right)
\end{equation}
\begin{equation}
-{\beta} {{p\!H}} {\sigma} {\mathrm{E}_{t}\left[\lambda^{\mathrm{HIGHREGIME}^{\mathrm{2}}}_{t+1}\right]} = 0
 \quad \left({i\!H}_{t}\right)
\end{equation}




\section{LOWREGIME}

\subsection{Optimisation problem}

\begin{align}
&\max_{{p\!i\!L}_{t}, {y\!L}_{t}, {i\!L}_{t}
} {U\!L}_{t} = -0.5{{p\!i\!L}_{t}}^{2} + {\beta} \left({{p\!L}} {\mathrm{E}_{t}\left[{U\!L}_{t+1}\right]} + \left(1 - {p\!L}\right) {\mathrm{E}_{t}\left[{U\!H}_{t+1}\right]}\right) - 0.5{\kappa} {\theta}^{-1} {{y\!L}_{t}}^{2}\\
&\mathrm{s.t.:}\nonumber\\
& {p\!i\!L}_{t-1} = {\beta} \left({{p\!L}} {{p\!i\!L}_{t}} + {{p\!i\!H}_{t}} \left(1 - {p\!L}\right)\right) + {\kappa} {{y\!L}_{t-1}} \quad \left(\lambda^{\mathrm{LOWREGIME}^{\mathrm{1}}}_{t}\right)\\
& {y\!L}_{t-1} = {{p\!L}} {{y\!L}_{t}} + {{y\!H}_{t}} \left(1 - {p\!L}\right) - {\sigma} \left({i\!L}_{t-1} - {r\!n}_{t-1} - {{p\!L}} {{p\!i\!L}_{t}} - {{p\!i\!H}_{t}} \left(1 - {p\!L}\right)\right) \quad \left(\lambda^{\mathrm{LOWREGIME}^{\mathrm{2}}}_{t}\right)
\end{align}


\subsection{First order conditions}

\begin{equation}
-{p\!i\!L}_{t} + {\beta} {{p\!L}} {\lambda^{\mathrm{LOWREGIME}^{\mathrm{1}}}_{t}} - {\beta} {{p\!L}} {\mathrm{E}_{t}\left[\lambda^{\mathrm{LOWREGIME}^{\mathrm{1}}}_{t+1}\right]} + {{p\!L}} {\sigma} {\lambda^{\mathrm{LOWREGIME}^{\mathrm{2}}}_{t}} = 0
 \quad \left({p\!i\!L}_{t}\right)
\end{equation}
\begin{equation}
{{p\!L}} {\lambda^{\mathrm{LOWREGIME}^{\mathrm{2}}}_{t}} + {\beta} {{p\!L}} \left({\kappa} {\mathrm{E}_{t}\left[\lambda^{\mathrm{LOWREGIME}^{\mathrm{1}}}_{t+1}\right]} - \mathrm{E}_{t}\left[\lambda^{\mathrm{LOWREGIME}^{\mathrm{2}}}_{t+1}\right]\right) - {\kappa} {\theta}^{-1} {{y\!L}_{t}} = 0
 \quad \left({y\!L}_{t}\right)
\end{equation}
\begin{equation}
-{\beta} {{p\!L}} {\sigma} {\mathrm{E}_{t}\left[\lambda^{\mathrm{LOWREGIME}^{\mathrm{2}}}_{t+1}\right]} = 0
 \quad \left({i\!L}_{t}\right)
\end{equation}




\section{EXOG}

\subsection{Identities}

\begin{equation}
{r\!n}_{t} = e^{\epsilon^{\mathrm{Z}}_{t} + {\phi} {\log{{r\!n}_{t-1}}}}
\end{equation}




\section{Equilibrium relationships (after reduction)}

\begin{equation}
-{r\!n}_{t} + e^{\epsilon^{\mathrm{Z}}_{t} + {\phi} {\log{{r\!n}_{t-1}}}} = 0
\end{equation}
\begin{equation}
-{p\!i\!H}_{t-1} + {\beta} \left({{p\!H}} {{p\!i\!H}_{t}} + {{p\!i\!L}_{t}} \left(1 - {p\!H}\right)\right) + {\kappa} {{y\!H}_{t-1}} = 0
\end{equation}
\begin{equation}
-{p\!i\!L}_{t-1} + {\beta} \left({{p\!L}} {{p\!i\!L}_{t}} + {{p\!i\!H}_{t}} \left(1 - {p\!L}\right)\right) + {\kappa} {{y\!L}_{t-1}} = 0
\end{equation}
\begin{equation}
{{p\!H}} {\lambda^{\mathrm{HIGHREGIME}^{\mathrm{2}}}_{t}} + {\beta} {{p\!H}} \left({\kappa} {\mathrm{E}_{t}\left[\lambda^{\mathrm{HIGHREGIME}^{\mathrm{1}}}_{t+1}\right]} - \mathrm{E}_{t}\left[\lambda^{\mathrm{HIGHREGIME}^{\mathrm{2}}}_{t+1}\right]\right) - {\kappa} {\theta}^{-1} {{y\!H}_{t}} = 0
\end{equation}
\begin{equation}
{{p\!L}} {\lambda^{\mathrm{LOWREGIME}^{\mathrm{2}}}_{t}} + {\beta} {{p\!L}} \left({\kappa} {\mathrm{E}_{t}\left[\lambda^{\mathrm{LOWREGIME}^{\mathrm{1}}}_{t+1}\right]} - \mathrm{E}_{t}\left[\lambda^{\mathrm{LOWREGIME}^{\mathrm{2}}}_{t+1}\right]\right) - {\kappa} {\theta}^{-1} {{y\!L}_{t}} = 0
\end{equation}
\begin{equation}
-{y\!H}_{t-1} + {{p\!H}} {{y\!H}_{t}} - {\sigma} \left({i\!H}_{t-1} - {r\!n}_{t-1} - {{p\!H}} {{p\!i\!H}_{t}} - {{p\!i\!L}_{t}} \left(1 - {p\!H}\right)\right) + {{y\!L}_{t}} \left(1 - {p\!H}\right) = 0
\end{equation}
\begin{equation}
-{y\!L}_{t-1} + {{p\!L}} {{y\!L}_{t}} - {\sigma} \left({i\!L}_{t-1} - {r\!n}_{t-1} - {{p\!L}} {{p\!i\!L}_{t}} - {{p\!i\!H}_{t}} \left(1 - {p\!L}\right)\right) + {{y\!H}_{t}} \left(1 - {p\!L}\right) = 0
\end{equation}
\begin{equation}
-{p\!i\!H}_{t} + {\beta} {{p\!H}} {\lambda^{\mathrm{HIGHREGIME}^{\mathrm{1}}}_{t}} - {\beta} {{p\!H}} {\mathrm{E}_{t}\left[\lambda^{\mathrm{HIGHREGIME}^{\mathrm{1}}}_{t+1}\right]} + {{p\!H}} {\sigma} {\lambda^{\mathrm{HIGHREGIME}^{\mathrm{2}}}_{t}} = 0
\end{equation}
\begin{equation}
-{p\!i\!L}_{t} + {\beta} {{p\!L}} {\lambda^{\mathrm{LOWREGIME}^{\mathrm{1}}}_{t}} - {\beta} {{p\!L}} {\mathrm{E}_{t}\left[\lambda^{\mathrm{LOWREGIME}^{\mathrm{1}}}_{t+1}\right]} + {{p\!L}} {\sigma} {\lambda^{\mathrm{LOWREGIME}^{\mathrm{2}}}_{t}} = 0
\end{equation}
\begin{equation}
{U\!H}_{t} + 0.5{{p\!i\!H}_{t}}^{2} - {\beta} \left({{p\!H}} {\mathrm{E}_{t}\left[{U\!H}_{t+1}\right]} + \left(1 - {p\!H}\right) {\mathrm{E}_{t}\left[{U\!L}_{t+1}\right]}\right) + 0.5{\kappa} {\theta}^{-1} {{y\!H}_{t}}^{2} = 0
\end{equation}
\begin{equation}
{U\!L}_{t} + 0.5{{p\!i\!L}_{t}}^{2} - {\beta} \left({{p\!L}} {\mathrm{E}_{t}\left[{U\!L}_{t+1}\right]} + \left(1 - {p\!L}\right) {\mathrm{E}_{t}\left[{U\!H}_{t+1}\right]}\right) + 0.5{\kappa} {\theta}^{-1} {{y\!L}_{t}}^{2} = 0
\end{equation}
\begin{equation}
-{\beta} {{p\!H}} {\sigma} {\mathrm{E}_{t}\left[\lambda^{\mathrm{HIGHREGIME}^{\mathrm{2}}}_{t+1}\right]} = 0
\end{equation}
\begin{equation}
-{\beta} {{p\!L}} {\sigma} {\mathrm{E}_{t}\left[\lambda^{\mathrm{LOWREGIME}^{\mathrm{2}}}_{t+1}\right]} = 0
\end{equation}



\section{Steady state relationships (after reduction)}

\begin{equation}
-{r\!n}_\mathrm{ss} + e^{{\phi} {\log{{r\!n}_\mathrm{ss}}}} = 0
\end{equation}
\begin{equation}
-{p\!i\!H}_\mathrm{ss} + {\beta} \left({{p\!H}} {{p\!i\!H}_\mathrm{ss}} + {{p\!i\!L}_\mathrm{ss}} \left(1 - {p\!H}\right)\right) + {\kappa} {{y\!H}_\mathrm{ss}} = 0
\end{equation}
\begin{equation}
-{p\!i\!L}_\mathrm{ss} + {\beta} \left({{p\!L}} {{p\!i\!L}_\mathrm{ss}} + {{p\!i\!H}_\mathrm{ss}} \left(1 - {p\!L}\right)\right) + {\kappa} {{y\!L}_\mathrm{ss}} = 0
\end{equation}
\begin{equation}
{{p\!H}} {\lambda^{\mathrm{HIGHREGIME}^{\mathrm{2}}}_\mathrm{ss}} + {\beta} {{p\!H}} \left(-\lambda^{\mathrm{HIGHREGIME}^{\mathrm{2}}}_\mathrm{ss} + {\kappa} {\lambda^{\mathrm{HIGHREGIME}^{\mathrm{1}}}_\mathrm{ss}}\right) - {\kappa} {\theta}^{-1} {{y\!H}_\mathrm{ss}} = 0
\end{equation}
\begin{equation}
{{p\!L}} {\lambda^{\mathrm{LOWREGIME}^{\mathrm{2}}}_\mathrm{ss}} + {\beta} {{p\!L}} \left(-\lambda^{\mathrm{LOWREGIME}^{\mathrm{2}}}_\mathrm{ss} + {\kappa} {\lambda^{\mathrm{LOWREGIME}^{\mathrm{1}}}_\mathrm{ss}}\right) - {\kappa} {\theta}^{-1} {{y\!L}_\mathrm{ss}} = 0
\end{equation}
\begin{equation}
-{y\!H}_\mathrm{ss} + {{p\!H}} {{y\!H}_\mathrm{ss}} - {\sigma} \left({i\!H}_\mathrm{ss} - {r\!n}_\mathrm{ss} - {{p\!H}} {{p\!i\!H}_\mathrm{ss}} - {{p\!i\!L}_\mathrm{ss}} \left(1 - {p\!H}\right)\right) + {{y\!L}_\mathrm{ss}} \left(1 - {p\!H}\right) = 0
\end{equation}
\begin{equation}
-{y\!L}_\mathrm{ss} + {{p\!L}} {{y\!L}_\mathrm{ss}} - {\sigma} \left({i\!L}_\mathrm{ss} - {r\!n}_\mathrm{ss} - {{p\!L}} {{p\!i\!L}_\mathrm{ss}} - {{p\!i\!H}_\mathrm{ss}} \left(1 - {p\!L}\right)\right) + {{y\!H}_\mathrm{ss}} \left(1 - {p\!L}\right) = 0
\end{equation}
\begin{equation}
-{p\!i\!H}_\mathrm{ss} + {{p\!H}} {\sigma} {\lambda^{\mathrm{HIGHREGIME}^{\mathrm{2}}}_\mathrm{ss}} = 0
\end{equation}
\begin{equation}
-{p\!i\!L}_\mathrm{ss} + {{p\!L}} {\sigma} {\lambda^{\mathrm{LOWREGIME}^{\mathrm{2}}}_\mathrm{ss}} = 0
\end{equation}
\begin{equation}
{U\!H}_\mathrm{ss} + 0.5{{p\!i\!H}_\mathrm{ss}}^{2} - {\beta} \left({{p\!H}} {{U\!H}_\mathrm{ss}} + {{U\!L}_\mathrm{ss}} \left(1 - {p\!H}\right)\right) + 0.5{\kappa} {\theta}^{-1} {{y\!H}_\mathrm{ss}}^{2} = 0
\end{equation}
\begin{equation}
{U\!L}_\mathrm{ss} + 0.5{{p\!i\!L}_\mathrm{ss}}^{2} - {\beta} \left({{p\!L}} {{U\!L}_\mathrm{ss}} + {{U\!H}_\mathrm{ss}} \left(1 - {p\!L}\right)\right) + 0.5{\kappa} {\theta}^{-1} {{y\!L}_\mathrm{ss}}^{2} = 0
\end{equation}
\begin{equation}
-{\beta} {{p\!H}} {\sigma} {\lambda^{\mathrm{HIGHREGIME}^{\mathrm{2}}}_\mathrm{ss}} = 0
\end{equation}
\begin{equation}
-{\beta} {{p\!L}} {\sigma} {\lambda^{\mathrm{LOWREGIME}^{\mathrm{2}}}_\mathrm{ss}} = 0
\end{equation}






\section{Parameter settings}

\begin{equation}
\beta = 0.99
\end{equation}
\begin{equation}
\kappa = 0.2465
\end{equation}
\begin{equation}
\phi = 0.95
\end{equation}
\begin{equation}
{p\!H} = 0.99
\end{equation}
\begin{equation}
{p\!L} = 0.99
\end{equation}
\begin{equation}
\sigma = 1
\end{equation}
\begin{equation}
\theta = 6
\end{equation}


