% Generated on 2023-11-21 15:47:37 by gEcon ver. 1.2.1 (2023-01-18)
% http://gecon.r-forge.r-project.org/

% Model name: RSW_RP

\section{HIGHREGIME}

\subsection{Optimisation problem}

\begin{align}
&\max_{{p\!i\!H}_{t}, {y\!H}_{t}, {i\!H}_{t}
} {U\!H}_{t} = -0.5\left({p\!i\!t\!H} - {p\!i\!t\!C\!B} + {p\!i\!H}_{t}\right)^{2} + {\beta} {\mathrm{E}_{t}\left[{U\!H}_{t+1}\right]} + {\beta} \left(1 - {p\!H}\right) \left(-\mathrm{E}_{t}\left[{U\!H}_{t+1}\right] + \mathrm{E}_{t}\left[{U\!L}_{t+1}\right]\right) - 0.5{\kappa} {\theta}^{-1} {{y\!H}_{t}}^{2}\\
&\mathrm{s.t.:}\nonumber\\
& {p\!i\!H}_{t-1} = \log{{e\!t\!a\!p\!i}_{t-1}} + {\beta} {{p\!i\!H}_{t}} + {\kappa} {{y\!H}_{t-1}} + {\beta} \left(1 - {p\!H}\right) \left(-{p\!i\!H}_{t} + {p\!i\!L}_{t}\right) \quad \left(\lambda^{\mathrm{HIGHREGIME}^{\mathrm{1}}}_{t}\right)\\
& {y\!H}_{t-1} = {y\!H}_{t} - {\sigma} \left({i\!H}_{t-1} - {p\!i\!H}_{t}\right) + \left(1 - {p\!H}\right) \left(-{y\!H}_{t} + {y\!L}_{t}\right) + {\sigma} \left(1 - {p\!H}\right) \left(-{p\!i\!H}_{t} + {p\!i\!L}_{t}\right) \quad \left(\lambda^{\mathrm{HIGHREGIME}^{\mathrm{2}}}_{t}\right)
\end{align}


\subsection{First order conditions}

\begin{equation}
-{p\!i\!t\!H} + {p\!i\!t\!C\!B} - {p\!i\!H}_{t} + {\lambda^{\mathrm{HIGHREGIME}^{\mathrm{1}}}_{t}} \left(\beta - {\beta} \left(1 - {p\!H}\right)\right) + {\lambda^{\mathrm{HIGHREGIME}^{\mathrm{2}}}_{t}} \left(\sigma - {\sigma} \left(1 - {p\!H}\right)\right) - \left(\beta - {\beta} \left(1 - {p\!H}\right)\right) {\mathrm{E}_{t}\left[\lambda^{\mathrm{HIGHREGIME}^{\mathrm{1}}}_{t+1}\right]} = 0
 \quad \left({p\!i\!H}_{t}\right)
\end{equation}
\begin{equation}
{{p\!H}} {\lambda^{\mathrm{HIGHREGIME}^{\mathrm{2}}}_{t}} + \left(\beta - {\beta} \left(1 - {p\!H}\right)\right) \left({\kappa} {\mathrm{E}_{t}\left[\lambda^{\mathrm{HIGHREGIME}^{\mathrm{1}}}_{t+1}\right]} - \mathrm{E}_{t}\left[\lambda^{\mathrm{HIGHREGIME}^{\mathrm{2}}}_{t+1}\right]\right) - {\kappa} {\theta}^{-1} {{y\!H}_{t}} = 0
 \quad \left({y\!H}_{t}\right)
\end{equation}
\begin{equation}
-{\sigma} \left(\beta - {\beta} \left(1 - {p\!H}\right)\right) {\mathrm{E}_{t}\left[\lambda^{\mathrm{HIGHREGIME}^{\mathrm{2}}}_{t+1}\right]} = 0
 \quad \left({i\!H}_{t}\right)
\end{equation}




\section{LOWREGIME}

\subsection{Optimisation problem}

\begin{align}
&\max_{{p\!i\!L}_{t}, {y\!L}_{t}, {i\!L}_{t}
} {U\!L}_{t} = -0.5\left(-{p\!i\!t\!C\!B} + {p\!i\!t\!L} + {p\!i\!L}_{t}\right)^{2} + {\beta} {\mathrm{E}_{t}\left[{U\!L}_{t+1}\right]} + {\beta} \left(1 - {p\!L}\right) \left(\mathrm{E}_{t}\left[{U\!H}_{t+1}\right] - \mathrm{E}_{t}\left[{U\!L}_{t+1}\right]\right) - 0.5{\kappa} {\theta}^{-1} {{y\!L}_{t}}^{2}\\
&\mathrm{s.t.:}\nonumber\\
& {p\!i\!L}_{t-1} = \log{{e\!t\!a\!p\!i}_{t-1}} + {\kappa} {{y\!L}_{t-1}} + {\beta} {{p\!L}} {{p\!i\!L}_{t}} + {\beta} \left(1 - {p\!L}\right) \left({p\!i\!H}_{t} - {p\!i\!L}_{t}\right) \quad \left(\lambda^{\mathrm{LOWREGIME}^{\mathrm{1}}}_{t}\right)\\
& {y\!L}_{t-1} = {y\!L}_{t} - {\sigma} \left({i\!L}_{t-1} - {p\!i\!L}_{t}\right) + \left(1 - {p\!L}\right) \left({y\!H}_{t} - {y\!L}_{t}\right) + {\sigma} \left(1 - {p\!L}\right) \left({p\!i\!H}_{t} - {p\!i\!L}_{t}\right) \quad \left(\lambda^{\mathrm{LOWREGIME}^{\mathrm{2}}}_{t}\right)
\end{align}


\subsection{First order conditions}

\begin{equation}
{p\!i\!t\!C\!B} - {p\!i\!t\!L} - {p\!i\!L}_{t} + {\lambda^{\mathrm{LOWREGIME}^{\mathrm{1}}}_{t}} \left({\beta} {{p\!L}} - {\beta} \left(1 - {p\!L}\right)\right) + {\lambda^{\mathrm{LOWREGIME}^{\mathrm{2}}}_{t}} \left(\sigma - {\sigma} \left(1 - {p\!L}\right)\right) - \left(\beta - {\beta} \left(1 - {p\!L}\right)\right) {\mathrm{E}_{t}\left[\lambda^{\mathrm{LOWREGIME}^{\mathrm{1}}}_{t+1}\right]} = 0
 \quad \left({p\!i\!L}_{t}\right)
\end{equation}
\begin{equation}
{{p\!L}} {\lambda^{\mathrm{LOWREGIME}^{\mathrm{2}}}_{t}} + \left(\beta - {\beta} \left(1 - {p\!L}\right)\right) \left({\kappa} {\mathrm{E}_{t}\left[\lambda^{\mathrm{LOWREGIME}^{\mathrm{1}}}_{t+1}\right]} - \mathrm{E}_{t}\left[\lambda^{\mathrm{LOWREGIME}^{\mathrm{2}}}_{t+1}\right]\right) - {\kappa} {\theta}^{-1} {{y\!L}_{t}} = 0
 \quad \left({y\!L}_{t}\right)
\end{equation}
\begin{equation}
-{\sigma} \left(\beta - {\beta} \left(1 - {p\!L}\right)\right) {\mathrm{E}_{t}\left[\lambda^{\mathrm{LOWREGIME}^{\mathrm{2}}}_{t+1}\right]} = 0
 \quad \left({i\!L}_{t}\right)
\end{equation}




\section{EXOG}

\subsection{Identities}

\begin{equation}
{e\!t\!a\!p\!i}_{t} = e^{\epsilon^{\pi}_{t} + {\phi} {\log{{e\!t\!a\!p\!i}_{t-1}}}}
\end{equation}




\section{Equilibrium relationships (after reduction)}

\begin{equation}
-{e\!t\!a\!p\!i}_{t} + e^{\epsilon^{\pi}_{t} + {\phi} {\log{{e\!t\!a\!p\!i}_{t-1}}}} = 0
\end{equation}
\begin{equation}
{{p\!H}} {\lambda^{\mathrm{HIGHREGIME}^{\mathrm{2}}}_{t}} + \left(\beta - {\beta} \left(1 - {p\!H}\right)\right) \left({\kappa} {\mathrm{E}_{t}\left[\lambda^{\mathrm{HIGHREGIME}^{\mathrm{1}}}_{t+1}\right]} - \mathrm{E}_{t}\left[\lambda^{\mathrm{HIGHREGIME}^{\mathrm{2}}}_{t+1}\right]\right) - {\kappa} {\theta}^{-1} {{y\!H}_{t}} = 0
\end{equation}
\begin{equation}
{{p\!L}} {\lambda^{\mathrm{LOWREGIME}^{\mathrm{2}}}_{t}} + \left(\beta - {\beta} \left(1 - {p\!L}\right)\right) \left({\kappa} {\mathrm{E}_{t}\left[\lambda^{\mathrm{LOWREGIME}^{\mathrm{1}}}_{t+1}\right]} - \mathrm{E}_{t}\left[\lambda^{\mathrm{LOWREGIME}^{\mathrm{2}}}_{t+1}\right]\right) - {\kappa} {\theta}^{-1} {{y\!L}_{t}} = 0
\end{equation}
\begin{equation}
-{p\!i\!H}_{t-1} + \log{{e\!t\!a\!p\!i}_{t-1}} + {\beta} {{p\!i\!H}_{t}} + {\kappa} {{y\!H}_{t-1}} + {\beta} \left(1 - {p\!H}\right) \left(-{p\!i\!H}_{t} + {p\!i\!L}_{t}\right) = 0
\end{equation}
\begin{equation}
-{p\!i\!L}_{t-1} + \log{{e\!t\!a\!p\!i}_{t-1}} + {\kappa} {{y\!L}_{t-1}} + {\beta} {{p\!L}} {{p\!i\!L}_{t}} + {\beta} \left(1 - {p\!L}\right) \left({p\!i\!H}_{t} - {p\!i\!L}_{t}\right) = 0
\end{equation}
\begin{equation}
-{y\!H}_{t-1} + {y\!H}_{t} - {\sigma} \left({i\!H}_{t-1} - {p\!i\!H}_{t}\right) + \left(1 - {p\!H}\right) \left(-{y\!H}_{t} + {y\!L}_{t}\right) + {\sigma} \left(1 - {p\!H}\right) \left(-{p\!i\!H}_{t} + {p\!i\!L}_{t}\right) = 0
\end{equation}
\begin{equation}
-{y\!L}_{t-1} + {y\!L}_{t} - {\sigma} \left({i\!L}_{t-1} - {p\!i\!L}_{t}\right) + \left(1 - {p\!L}\right) \left({y\!H}_{t} - {y\!L}_{t}\right) + {\sigma} \left(1 - {p\!L}\right) \left({p\!i\!H}_{t} - {p\!i\!L}_{t}\right) = 0
\end{equation}
\begin{equation}
{U\!H}_{t} + 0.5\left({p\!i\!t\!H} - {p\!i\!t\!C\!B} + {p\!i\!H}_{t}\right)^{2} - {\beta} {\mathrm{E}_{t}\left[{U\!H}_{t+1}\right]} - {\beta} \left(1 - {p\!H}\right) \left(-\mathrm{E}_{t}\left[{U\!H}_{t+1}\right] + \mathrm{E}_{t}\left[{U\!L}_{t+1}\right]\right) + 0.5{\kappa} {\theta}^{-1} {{y\!H}_{t}}^{2} = 0
\end{equation}
\begin{equation}
{U\!L}_{t} + 0.5\left(-{p\!i\!t\!C\!B} + {p\!i\!t\!L} + {p\!i\!L}_{t}\right)^{2} - {\beta} {\mathrm{E}_{t}\left[{U\!L}_{t+1}\right]} - {\beta} \left(1 - {p\!L}\right) \left(\mathrm{E}_{t}\left[{U\!H}_{t+1}\right] - \mathrm{E}_{t}\left[{U\!L}_{t+1}\right]\right) + 0.5{\kappa} {\theta}^{-1} {{y\!L}_{t}}^{2} = 0
\end{equation}
\begin{equation}
-{p\!i\!t\!H} + {p\!i\!t\!C\!B} - {p\!i\!H}_{t} + {\lambda^{\mathrm{HIGHREGIME}^{\mathrm{1}}}_{t}} \left(\beta - {\beta} \left(1 - {p\!H}\right)\right) + {\lambda^{\mathrm{HIGHREGIME}^{\mathrm{2}}}_{t}} \left(\sigma - {\sigma} \left(1 - {p\!H}\right)\right) - \left(\beta - {\beta} \left(1 - {p\!H}\right)\right) {\mathrm{E}_{t}\left[\lambda^{\mathrm{HIGHREGIME}^{\mathrm{1}}}_{t+1}\right]} = 0
\end{equation}
\begin{equation}
{p\!i\!t\!C\!B} - {p\!i\!t\!L} - {p\!i\!L}_{t} + {\lambda^{\mathrm{LOWREGIME}^{\mathrm{1}}}_{t}} \left({\beta} {{p\!L}} - {\beta} \left(1 - {p\!L}\right)\right) + {\lambda^{\mathrm{LOWREGIME}^{\mathrm{2}}}_{t}} \left(\sigma - {\sigma} \left(1 - {p\!L}\right)\right) - \left(\beta - {\beta} \left(1 - {p\!L}\right)\right) {\mathrm{E}_{t}\left[\lambda^{\mathrm{LOWREGIME}^{\mathrm{1}}}_{t+1}\right]} = 0
\end{equation}
\begin{equation}
-{\sigma} \left(\beta - {\beta} \left(1 - {p\!H}\right)\right) {\mathrm{E}_{t}\left[\lambda^{\mathrm{HIGHREGIME}^{\mathrm{2}}}_{t+1}\right]} = 0
\end{equation}
\begin{equation}
-{\sigma} \left(\beta - {\beta} \left(1 - {p\!L}\right)\right) {\mathrm{E}_{t}\left[\lambda^{\mathrm{LOWREGIME}^{\mathrm{2}}}_{t+1}\right]} = 0
\end{equation}



\section{Steady state relationships (after reduction)}

\begin{equation}
-{e\!t\!a\!p\!i}_\mathrm{ss} + e^{{\phi} {\log{{e\!t\!a\!p\!i}_\mathrm{ss}}}} = 0
\end{equation}
\begin{equation}
{{p\!H}} {\lambda^{\mathrm{HIGHREGIME}^{\mathrm{2}}}_\mathrm{ss}} + \left(\beta - {\beta} \left(1 - {p\!H}\right)\right) \left(-\lambda^{\mathrm{HIGHREGIME}^{\mathrm{2}}}_\mathrm{ss} + {\kappa} {\lambda^{\mathrm{HIGHREGIME}^{\mathrm{1}}}_\mathrm{ss}}\right) - {\kappa} {\theta}^{-1} {{y\!H}_\mathrm{ss}} = 0
\end{equation}
\begin{equation}
{{p\!L}} {\lambda^{\mathrm{LOWREGIME}^{\mathrm{2}}}_\mathrm{ss}} + \left(\beta - {\beta} \left(1 - {p\!L}\right)\right) \left(-\lambda^{\mathrm{LOWREGIME}^{\mathrm{2}}}_\mathrm{ss} + {\kappa} {\lambda^{\mathrm{LOWREGIME}^{\mathrm{1}}}_\mathrm{ss}}\right) - {\kappa} {\theta}^{-1} {{y\!L}_\mathrm{ss}} = 0
\end{equation}
\begin{equation}
-{p\!i\!H}_\mathrm{ss} + \log{{e\!t\!a\!p\!i}_\mathrm{ss}} + {\beta} {{p\!i\!H}_\mathrm{ss}} + {\kappa} {{y\!H}_\mathrm{ss}} + {\beta} \left(1 - {p\!H}\right) \left(-{p\!i\!H}_\mathrm{ss} + {p\!i\!L}_\mathrm{ss}\right) = 0
\end{equation}
\begin{equation}
-{p\!i\!L}_\mathrm{ss} + \log{{e\!t\!a\!p\!i}_\mathrm{ss}} + {\kappa} {{y\!L}_\mathrm{ss}} + {\beta} {{p\!L}} {{p\!i\!L}_\mathrm{ss}} + {\beta} \left(1 - {p\!L}\right) \left({p\!i\!H}_\mathrm{ss} - {p\!i\!L}_\mathrm{ss}\right) = 0
\end{equation}
\begin{equation}
\left(1 - {p\!H}\right) \left(-{y\!H}_\mathrm{ss} + {y\!L}_\mathrm{ss}\right) - {\sigma} \left({i\!H}_\mathrm{ss} - {p\!i\!H}_\mathrm{ss}\right) + {\sigma} \left(1 - {p\!H}\right) \left(-{p\!i\!H}_\mathrm{ss} + {p\!i\!L}_\mathrm{ss}\right) = 0
\end{equation}
\begin{equation}
\left(1 - {p\!L}\right) \left({y\!H}_\mathrm{ss} - {y\!L}_\mathrm{ss}\right) - {\sigma} \left({i\!L}_\mathrm{ss} - {p\!i\!L}_\mathrm{ss}\right) + {\sigma} \left(1 - {p\!L}\right) \left({p\!i\!H}_\mathrm{ss} - {p\!i\!L}_\mathrm{ss}\right) = 0
\end{equation}
\begin{equation}
{U\!H}_\mathrm{ss} + 0.5\left({p\!i\!t\!H} - {p\!i\!t\!C\!B} + {p\!i\!H}_\mathrm{ss}\right)^{2} - {\beta} {{U\!H}_\mathrm{ss}} - {\beta} \left(1 - {p\!H}\right) \left(-{U\!H}_\mathrm{ss} + {U\!L}_\mathrm{ss}\right) + 0.5{\kappa} {\theta}^{-1} {{y\!H}_\mathrm{ss}}^{2} = 0
\end{equation}
\begin{equation}
{U\!L}_\mathrm{ss} + 0.5\left(-{p\!i\!t\!C\!B} + {p\!i\!t\!L} + {p\!i\!L}_\mathrm{ss}\right)^{2} - {\beta} {{U\!L}_\mathrm{ss}} - {\beta} \left(1 - {p\!L}\right) \left({U\!H}_\mathrm{ss} - {U\!L}_\mathrm{ss}\right) + 0.5{\kappa} {\theta}^{-1} {{y\!L}_\mathrm{ss}}^{2} = 0
\end{equation}
\begin{equation}
-{p\!i\!t\!H} + {p\!i\!t\!C\!B} - {p\!i\!H}_\mathrm{ss} + {\lambda^{\mathrm{HIGHREGIME}^{\mathrm{2}}}_\mathrm{ss}} \left(\sigma - {\sigma} \left(1 - {p\!H}\right)\right) = 0
\end{equation}
\begin{equation}
{p\!i\!t\!C\!B} - {p\!i\!t\!L} - {p\!i\!L}_\mathrm{ss} - {\lambda^{\mathrm{LOWREGIME}^{\mathrm{1}}}_\mathrm{ss}} \left(\beta - {\beta} \left(1 - {p\!L}\right)\right) + {\lambda^{\mathrm{LOWREGIME}^{\mathrm{1}}}_\mathrm{ss}} \left({\beta} {{p\!L}} - {\beta} \left(1 - {p\!L}\right)\right) + {\lambda^{\mathrm{LOWREGIME}^{\mathrm{2}}}_\mathrm{ss}} \left(\sigma - {\sigma} \left(1 - {p\!L}\right)\right) = 0
\end{equation}
\begin{equation}
-{\sigma} {\lambda^{\mathrm{HIGHREGIME}^{\mathrm{2}}}_\mathrm{ss}} \left(\beta - {\beta} \left(1 - {p\!H}\right)\right) = 0
\end{equation}
\begin{equation}
-{\sigma} {\lambda^{\mathrm{LOWREGIME}^{\mathrm{2}}}_\mathrm{ss}} \left(\beta - {\beta} \left(1 - {p\!L}\right)\right) = 0
\end{equation}






\section{Parameter settings}

\begin{equation}
\beta = 0.99
\end{equation}
\begin{equation}
\kappa = 0.2465
\end{equation}
\begin{equation}
\phi = 0.95
\end{equation}
\begin{equation}
{p\!i\!t\!H} = 0
\end{equation}
\begin{equation}
{p\!i\!t\!C\!B} = 0
\end{equation}
\begin{equation}
{p\!i\!t\!L} = 2
\end{equation}
\begin{equation}
{p\!H} = 0.99
\end{equation}
\begin{equation}
{p\!L} = 0.99
\end{equation}
\begin{equation}
\sigma = 1
\end{equation}
\begin{equation}
\theta = 6
\end{equation}


