% Generated on 2023-10-27 10:45:21 by gEcon ver. 1.2.1 (2023-01-18)
% http://gecon.r-forge.r-project.org/

% Model name: RW

\section{RW}

\subsection{Optimisation problem}

\begin{align}
&\max_{\pi_{t}, y_{t}, i_{t}
} U_{t} = -0.5\left(-{p\!i\!s\!t\!a\!r} + \pi_{t}\right)^{2} + {\beta} {\mathrm{E}_{t}\left[U_{t+1}\right]} - 0.5{\kappa} {\theta}^{-1} {y_{t}}^{2}\\
&\mathrm{s.t.:}\nonumber\\
& \pi_{t-1} = {e\!t\!a\!p\!i}_{t-1} + {\beta} {\pi_{t}} + {\kappa} {y_{t-1}} \quad \left(\lambda^{\mathrm{RW}^{\mathrm{1}}}_{t}\right)\\
& y_{t-1} = y_{t} - {\sigma} \left(i_{t-1} - \pi_{t}\right) \quad \left(\lambda^{\mathrm{RW}^{\mathrm{2}}}_{t}\right)
\end{align}


\subsection{First order conditions}

\begin{equation}
{p\!i\!s\!t\!a\!r} - \pi_{t} + {\beta} {\lambda^{\mathrm{RW}^{\mathrm{1}}}_{t}} - {\beta} {\mathrm{E}_{t}\left[\lambda^{\mathrm{RW}^{\mathrm{1}}}_{t+1}\right]} + {\sigma} {\lambda^{\mathrm{RW}^{\mathrm{2}}}_{t}} = 0
 \quad \left(\pi_{t}\right)
\end{equation}
\begin{equation}
\lambda^{\mathrm{RW}^{\mathrm{2}}}_{t} + {\beta} \left({\kappa} {\mathrm{E}_{t}\left[\lambda^{\mathrm{RW}^{\mathrm{1}}}_{t+1}\right]} - \mathrm{E}_{t}\left[\lambda^{\mathrm{RW}^{\mathrm{2}}}_{t+1}\right]\right) - {\kappa} {\theta}^{-1} {y_{t}} = 0
 \quad \left(y_{t}\right)
\end{equation}
\begin{equation}
-{\beta} {\sigma} {\mathrm{E}_{t}\left[\lambda^{\mathrm{RW}^{\mathrm{2}}}_{t+1}\right]} = 0
 \quad \left(i_{t}\right)
\end{equation}




\section{EXOG}

\subsection{Identities}

\begin{equation}
{e\!t\!a\!p\!i}_{t} = e^{\epsilon^{\pi}_{t} + {\phi} {\log{{e\!t\!a\!p\!i}_{t-1}}}}
\end{equation}




\section{Equilibrium relationships (after reduction)}

\begin{equation}
-{e\!t\!a\!p\!i}_{t} + e^{\epsilon^{\pi}_{t} + {\phi} {\log{{e\!t\!a\!p\!i}_{t-1}}}} = 0
\end{equation}
\begin{equation}
-y_{t-1} + y_{t} - {\sigma} \left(i_{t-1} - \pi_{t}\right) = 0
\end{equation}
\begin{equation}
\lambda^{\mathrm{RW}^{\mathrm{2}}}_{t} + {\beta} \left({\kappa} {\mathrm{E}_{t}\left[\lambda^{\mathrm{RW}^{\mathrm{1}}}_{t+1}\right]} - \mathrm{E}_{t}\left[\lambda^{\mathrm{RW}^{\mathrm{2}}}_{t+1}\right]\right) - {\kappa} {\theta}^{-1} {y_{t}} = 0
\end{equation}
\begin{equation}
{e\!t\!a\!p\!i}_{t-1} - \pi_{t-1} + {\beta} {\pi_{t}} + {\kappa} {y_{t-1}} = 0
\end{equation}
\begin{equation}
U_{t} + 0.5\left(-{p\!i\!s\!t\!a\!r} + \pi_{t}\right)^{2} - {\beta} {\mathrm{E}_{t}\left[U_{t+1}\right]} + 0.5{\kappa} {\theta}^{-1} {y_{t}}^{2} = 0
\end{equation}
\begin{equation}
{p\!i\!s\!t\!a\!r} - \pi_{t} + {\beta} {\lambda^{\mathrm{RW}^{\mathrm{1}}}_{t}} - {\beta} {\mathrm{E}_{t}\left[\lambda^{\mathrm{RW}^{\mathrm{1}}}_{t+1}\right]} + {\sigma} {\lambda^{\mathrm{RW}^{\mathrm{2}}}_{t}} = 0
\end{equation}
\begin{equation}
-{\beta} {\sigma} {\mathrm{E}_{t}\left[\lambda^{\mathrm{RW}^{\mathrm{2}}}_{t+1}\right]} = 0
\end{equation}



\section{Steady state relationships (after reduction)}

\begin{equation}
-{e\!t\!a\!p\!i}_\mathrm{ss} + e^{{\phi} {\log{{e\!t\!a\!p\!i}_\mathrm{ss}}}} = 0
\end{equation}
\begin{equation}
-{\sigma} \left(i_\mathrm{ss} - \pi_\mathrm{ss}\right) = 0
\end{equation}
\begin{equation}
\lambda^{\mathrm{RW}^{\mathrm{2}}}_\mathrm{ss} + {\beta} \left(-\lambda^{\mathrm{RW}^{\mathrm{2}}}_\mathrm{ss} + {\kappa} {\lambda^{\mathrm{RW}^{\mathrm{1}}}_\mathrm{ss}}\right) - {\kappa} {\theta}^{-1} {y_\mathrm{ss}} = 0
\end{equation}
\begin{equation}
{e\!t\!a\!p\!i}_\mathrm{ss} - \pi_\mathrm{ss} + {\beta} {\pi_\mathrm{ss}} + {\kappa} {y_\mathrm{ss}} = 0
\end{equation}
\begin{equation}
U_\mathrm{ss} + 0.5\left(-{p\!i\!s\!t\!a\!r} + \pi_\mathrm{ss}\right)^{2} - {\beta} {U_\mathrm{ss}} + 0.5{\kappa} {\theta}^{-1} {y_\mathrm{ss}}^{2} = 0
\end{equation}
\begin{equation}
{p\!i\!s\!t\!a\!r} - \pi_\mathrm{ss} + {\sigma} {\lambda^{\mathrm{RW}^{\mathrm{2}}}_\mathrm{ss}} = 0
\end{equation}
\begin{equation}
-{\beta} {\sigma} {\lambda^{\mathrm{RW}^{\mathrm{2}}}_\mathrm{ss}} = 0
\end{equation}






\section{Parameter settings}

\begin{equation}
\beta = 0.99
\end{equation}
\begin{equation}
\kappa = 0.2465
\end{equation}
\begin{equation}
\phi = 0.95
\end{equation}
\begin{equation}
{p\!i\!s\!t\!a\!r} = 0
\end{equation}
\begin{equation}
\sigma = 1
\end{equation}
\begin{equation}
\theta = 6
\end{equation}


