% Generated on 2024-02-13 19:11:08 by gEcon ver. 1.2.1 (2023-01-18)
% http://gecon.r-forge.r-project.org/

% Model name: RSW_RP_ONEOBJ

\section{OPTIMALMP}

\subsection{Optimisation problem}

\begin{align}
&\max_{{p\!i\!H}_{t}, {y\!H}_{t}, {p\!i\!L}_{t}, {y\!L}_{t}
} U_{t} = -0.25\left({p\!i\!t\!H} - {p\!i\!t\!C\!B} + {p\!i\!H}_{t}\right)^{2} - 0.25\left(-{p\!i\!t\!C\!B} + {p\!i\!t\!L} + {p\!i\!L}_{t}\right)^{2} + {\beta} {\mathrm{E}_{t}\left[U_{t+1}\right]} - 0.25{\lambda} {{y\!H}_{t}}^{2} - 0.25{\lambda} {{y\!L}_{t}}^{2}\\
&\mathrm{s.t.:}\nonumber\\
& {p\!i\!H}_{t-1} = \log{{e\!t\!a\!p\!i}_{t-1}} + {\beta} {{p\!i\!H}_{t}} + {\kappa} {{y\!H}_{t-1}} + {\beta} \left(1 - {p\!H}\right) \left(-{p\!i\!H}_{t} + {p\!i\!L}_{t}\right) \quad \left(\lambda^{\mathrm{OPTIMALMP}^{\mathrm{1}}}_{t}\right)\\
& {p\!i\!L}_{t-1} = \log{{e\!t\!a\!p\!i}_{t-1}} + {\beta} {{p\!i\!L}_{t}} + {\kappa} {{y\!L}_{t-1}} + {\beta} \left(1 - {p\!L}\right) \left({p\!i\!H}_{t} - {p\!i\!L}_{t}\right) \quad \left(\lambda^{\mathrm{OPTIMALMP}^{\mathrm{2}}}_{t}\right)
\end{align}


\subsection{First order conditions}

\begin{equation}
-0.5{p\!i\!t\!H} + 0.5{p\!i\!t\!C\!B} - 0.5{p\!i\!H}_{t} - {\beta} {\mathrm{E}_{t}\left[\lambda^{\mathrm{OPTIMALMP}^{\mathrm{1}}}_{t+1}\right]} + {\lambda^{\mathrm{OPTIMALMP}^{\mathrm{1}}}_{t}} \left(\beta - {\beta} \left(1 - {p\!H}\right)\right) + {\beta} {\lambda^{\mathrm{OPTIMALMP}^{\mathrm{2}}}_{t}} \left(1 - {p\!L}\right) = 0
 \quad \left({p\!i\!H}_{t}\right)
\end{equation}
\begin{equation}
-0.5{\lambda} {{y\!H}_{t}} + {\beta} {\kappa} {\mathrm{E}_{t}\left[\lambda^{\mathrm{OPTIMALMP}^{\mathrm{1}}}_{t+1}\right]} = 0
 \quad \left({y\!H}_{t}\right)
\end{equation}
\begin{equation}
0.5{p\!i\!t\!C\!B} - 0.5{p\!i\!t\!L} - 0.5{p\!i\!L}_{t} - {\beta} {\mathrm{E}_{t}\left[\lambda^{\mathrm{OPTIMALMP}^{\mathrm{2}}}_{t+1}\right]} + {\lambda^{\mathrm{OPTIMALMP}^{\mathrm{2}}}_{t}} \left(\beta - {\beta} \left(1 - {p\!L}\right)\right) + {\beta} {\lambda^{\mathrm{OPTIMALMP}^{\mathrm{1}}}_{t}} \left(1 - {p\!H}\right) = 0
 \quad \left({p\!i\!L}_{t}\right)
\end{equation}
\begin{equation}
-0.5{\lambda} {{y\!L}_{t}} + {\beta} {\kappa} {\mathrm{E}_{t}\left[\lambda^{\mathrm{OPTIMALMP}^{\mathrm{2}}}_{t+1}\right]} = 0
 \quad \left({y\!L}_{t}\right)
\end{equation}




\section{EXOG}

\subsection{Identities}

\begin{equation}
{e\!t\!a\!p\!i}_{t} = e^{\epsilon^{\pi}_{t} + {\phi} {\log{{e\!t\!a\!p\!i}_{t-1}}}}
\end{equation}




\section{Equilibrium relationships (after reduction)}

\begin{equation}
-{e\!t\!a\!p\!i}_{t} + e^{\epsilon^{\pi}_{t} + {\phi} {\log{{e\!t\!a\!p\!i}_{t-1}}}} = 0
\end{equation}
\begin{equation}
-0.5{\lambda} {{y\!H}_{t}} + {\beta} {\kappa} {\mathrm{E}_{t}\left[\lambda^{\mathrm{OPTIMALMP}^{\mathrm{1}}}_{t+1}\right]} = 0
\end{equation}
\begin{equation}
-0.5{\lambda} {{y\!L}_{t}} + {\beta} {\kappa} {\mathrm{E}_{t}\left[\lambda^{\mathrm{OPTIMALMP}^{\mathrm{2}}}_{t+1}\right]} = 0
\end{equation}
\begin{equation}
-{p\!i\!H}_{t-1} + \log{{e\!t\!a\!p\!i}_{t-1}} + {\beta} {{p\!i\!H}_{t}} + {\kappa} {{y\!H}_{t-1}} + {\beta} \left(1 - {p\!H}\right) \left(-{p\!i\!H}_{t} + {p\!i\!L}_{t}\right) = 0
\end{equation}
\begin{equation}
-{p\!i\!L}_{t-1} + \log{{e\!t\!a\!p\!i}_{t-1}} + {\beta} {{p\!i\!L}_{t}} + {\kappa} {{y\!L}_{t-1}} + {\beta} \left(1 - {p\!L}\right) \left({p\!i\!H}_{t} - {p\!i\!L}_{t}\right) = 0
\end{equation}
\begin{equation}
-0.5{p\!i\!t\!H} + 0.5{p\!i\!t\!C\!B} - 0.5{p\!i\!H}_{t} - {\beta} {\mathrm{E}_{t}\left[\lambda^{\mathrm{OPTIMALMP}^{\mathrm{1}}}_{t+1}\right]} + {\lambda^{\mathrm{OPTIMALMP}^{\mathrm{1}}}_{t}} \left(\beta - {\beta} \left(1 - {p\!H}\right)\right) + {\beta} {\lambda^{\mathrm{OPTIMALMP}^{\mathrm{2}}}_{t}} \left(1 - {p\!L}\right) = 0
\end{equation}
\begin{equation}
0.5{p\!i\!t\!C\!B} - 0.5{p\!i\!t\!L} - 0.5{p\!i\!L}_{t} - {\beta} {\mathrm{E}_{t}\left[\lambda^{\mathrm{OPTIMALMP}^{\mathrm{2}}}_{t+1}\right]} + {\lambda^{\mathrm{OPTIMALMP}^{\mathrm{2}}}_{t}} \left(\beta - {\beta} \left(1 - {p\!L}\right)\right) + {\beta} {\lambda^{\mathrm{OPTIMALMP}^{\mathrm{1}}}_{t}} \left(1 - {p\!H}\right) = 0
\end{equation}
\begin{equation}
U_{t} + 0.25\left({p\!i\!t\!H} - {p\!i\!t\!C\!B} + {p\!i\!H}_{t}\right)^{2} + 0.25\left(-{p\!i\!t\!C\!B} + {p\!i\!t\!L} + {p\!i\!L}_{t}\right)^{2} - {\beta} {\mathrm{E}_{t}\left[U_{t+1}\right]} + 0.25{\lambda} {{y\!H}_{t}}^{2} + 0.25{\lambda} {{y\!L}_{t}}^{2} = 0
\end{equation}



\section{Steady state relationships (after reduction)}

\begin{equation}
-{e\!t\!a\!p\!i}_\mathrm{ss} + e^{{\phi} {\log{{e\!t\!a\!p\!i}_\mathrm{ss}}}} = 0
\end{equation}
\begin{equation}
-0.5{\lambda} {{y\!H}_\mathrm{ss}} + {\beta} {\kappa} {\lambda^{\mathrm{OPTIMALMP}^{\mathrm{1}}}_\mathrm{ss}} = 0
\end{equation}
\begin{equation}
-0.5{\lambda} {{y\!L}_\mathrm{ss}} + {\beta} {\kappa} {\lambda^{\mathrm{OPTIMALMP}^{\mathrm{2}}}_\mathrm{ss}} = 0
\end{equation}
\begin{equation}
-{p\!i\!H}_\mathrm{ss} + \log{{e\!t\!a\!p\!i}_\mathrm{ss}} + {\beta} {{p\!i\!H}_\mathrm{ss}} + {\kappa} {{y\!H}_\mathrm{ss}} + {\beta} \left(1 - {p\!H}\right) \left(-{p\!i\!H}_\mathrm{ss} + {p\!i\!L}_\mathrm{ss}\right) = 0
\end{equation}
\begin{equation}
-{p\!i\!L}_\mathrm{ss} + \log{{e\!t\!a\!p\!i}_\mathrm{ss}} + {\beta} {{p\!i\!L}_\mathrm{ss}} + {\kappa} {{y\!L}_\mathrm{ss}} + {\beta} \left(1 - {p\!L}\right) \left({p\!i\!H}_\mathrm{ss} - {p\!i\!L}_\mathrm{ss}\right) = 0
\end{equation}
\begin{equation}
-0.5{p\!i\!t\!H} + 0.5{p\!i\!t\!C\!B} - 0.5{p\!i\!H}_\mathrm{ss} - {\beta} {\lambda^{\mathrm{OPTIMALMP}^{\mathrm{1}}}_\mathrm{ss}} + {\lambda^{\mathrm{OPTIMALMP}^{\mathrm{1}}}_\mathrm{ss}} \left(\beta - {\beta} \left(1 - {p\!H}\right)\right) + {\beta} {\lambda^{\mathrm{OPTIMALMP}^{\mathrm{2}}}_\mathrm{ss}} \left(1 - {p\!L}\right) = 0
\end{equation}
\begin{equation}
0.5{p\!i\!t\!C\!B} - 0.5{p\!i\!t\!L} - 0.5{p\!i\!L}_\mathrm{ss} - {\beta} {\lambda^{\mathrm{OPTIMALMP}^{\mathrm{2}}}_\mathrm{ss}} + {\lambda^{\mathrm{OPTIMALMP}^{\mathrm{2}}}_\mathrm{ss}} \left(\beta - {\beta} \left(1 - {p\!L}\right)\right) + {\beta} {\lambda^{\mathrm{OPTIMALMP}^{\mathrm{1}}}_\mathrm{ss}} \left(1 - {p\!H}\right) = 0
\end{equation}
\begin{equation}
U_\mathrm{ss} + 0.25\left({p\!i\!t\!H} - {p\!i\!t\!C\!B} + {p\!i\!H}_\mathrm{ss}\right)^{2} + 0.25\left(-{p\!i\!t\!C\!B} + {p\!i\!t\!L} + {p\!i\!L}_\mathrm{ss}\right)^{2} - {\beta} {U_\mathrm{ss}} + 0.25{\lambda} {{y\!H}_\mathrm{ss}}^{2} + 0.25{\lambda} {{y\!L}_\mathrm{ss}}^{2} = 0
\end{equation}






\section{Parameter settings}

\begin{equation}
\beta = 0.99
\end{equation}
\begin{equation}
\kappa = 0.2465
\end{equation}
\begin{equation}
\lambda = 0.04106
\end{equation}
\begin{equation}
\phi = 0.95
\end{equation}
\begin{equation}
{p\!i\!t\!H} = 2
\end{equation}
\begin{equation}
{p\!i\!t\!C\!B} = 2
\end{equation}
\begin{equation}
{p\!i\!t\!L} = 4
\end{equation}
\begin{equation}
{p\!H} = 0.99
\end{equation}
\begin{equation}
{p\!L} = 0.99
\end{equation}
\begin{equation}
\sigma = 1
\end{equation}
\begin{equation}
\theta = 6
\end{equation}


